libcrux-ml-kem/proofs/fstar/extraction/Libcrux_ml_kem.Constant_time_ops.fsti
@@ -4,9 +4,35 @@ open Core
 open FStar.Mul
 
 /// Return 1 if `value` is not zero and 0 otherwise.
-val inz (value: u8) : Prims.Pure u8 Prims.l_True (fun _ -> Prims.l_True)
+val inz (value: u8)
+    : Prims.Pure u8
+      Prims.l_True
+      (ensures
+        fun result ->
+          let result:u8 = result in
+          Hax_lib.implies (value =. 0uy <: bool)
+            (fun temp_0_ ->
+                let _:Prims.unit = temp_0_ in
+                result =. 0uy <: bool) &&
+          Hax_lib.implies (value <>. 0uy <: bool)
+            (fun temp_0_ ->
+                let _:Prims.unit = temp_0_ in
+                result =. 1uy <: bool))
 
-val is_non_zero (value: u8) : Prims.Pure u8 Prims.l_True (fun _ -> Prims.l_True)
+val is_non_zero (value: u8)
+    : Prims.Pure u8
+      Prims.l_True
+      (ensures
+        fun result ->
+          let result:u8 = result in
+          Hax_lib.implies (value =. 0uy <: bool)
+            (fun temp_0_ ->
+                let _:Prims.unit = temp_0_ in
+                result =. 0uy <: bool) &&
+          Hax_lib.implies (value <>. 0uy <: bool)
+            (fun temp_0_ ->
+                let _:Prims.unit = temp_0_ in
+                result =. 1uy <: bool))
 
 /// Return 1 if the bytes of `lhs` and `rhs` do not exactly
 /// match and 0 otherwise.
